Renamed Ord/ to Structures/ amd Reification/ into /Reflection. Put more basic things in RCCBase.v. Separated code for reflective tactics from the code implementing the structures on which these tactics work. Refactored TrichDec to be compatible with LinDec. Put tests in a separate directory. Proved over a half of the specification for htqs plus some lemmas. Started working on memoization — implemented it ad hc using lists and trees. Created the directory Thrash/ to hold guass what. Cleaned up Prints, Evals, Computes, Checks and Function warnings.

RCCBase.v
@@ -1,11 +1,33 @@
+Add Rec LoadPath "/home/zeimer/Code/Coq".
+
 Require Export FunctionalExtensionality.
 
-Ltac inv H := inversion H; subst.
+Require Export Bool.
+Require Export List.
+Export ListNotations.
+
+Require Export Arith.
+Require Export Omega.
+
+Require Export Equality.
+Require Export Eqdep.
+
+Require Export Sorting.Permutation.
+Require Export Sorting.InsertionSort.
+
+Set Implicit Arguments.
+
+Hint Constructors reflect.
+
+(* General useful tactics. *)
+(*Ltac inv H := inversion H; subst.*)
+Ltac inv H := inversion H; subst; clear H; auto.
 
 Ltac gen x := generalize dependent x.
 
 Ltac ext x := extensionality x.
 
+(* Tactics for easier induction. *)
 Ltac term_contains t x :=
 match t with
     | x => idtac
@@ -59,3 +81,68 @@ match type of H with
 end.
 
 Ltac ind H := try intros until H; gen_IH H; ind' H.
+
+(* Tactics for reification. *)
+Ltac inList x l :=
+match l with
+    | [] => false
+    | x :: _ => true
+    | _ :: ?l' => inList x l'
+end.
+
+Ltac addToList x l :=
+  let b := inList x l in
+match b with
+    | true => l
+    | false => constr:(x :: l)
+end.
+
+Ltac lookup x l :=
+match l with
+    | x :: _ => constr:(0)
+    | _ :: ?l' => let n := lookup x l' in constr:(S n)
+end.
+
+(* Environments. *)
+Definition Env (X : Type) : Type := list X.
+
+Definition holds (n : nat) (env : Env Prop) : Prop := nth n env False.
+
+Definition Proofs : Type := list nat.
+
+Fixpoint allTrue (env : Env Prop) (proofs : Proofs) : Prop :=
+match proofs with
+    | [] => True
+    | h :: t => holds h env /\ allTrue env t
+end.
+
+Theorem find_spec :
+  forall (n : nat) (env : Env Prop) (proofs : Proofs),
+    allTrue env proofs -> In n proofs -> holds n env.
+Proof.
+  induction proofs as [| h t]; cbn.
+    inversion 2.
+    do 2 destruct 1; subst.
+      unfold holds in H. apply H.
+      apply IHt; assumption.
+Qed.
+
+Inductive solution (P : Prop) : Type :=
+    | Yes' : P -> solution P
+    | No' : solution P.
+
+Arguments Yes' [P] _.
+Arguments No' [P].
+
+Notation "'Yes'" := (Yes' _).
+Notation "'No'" := No'.
+
+Notation "'Reduce' x" := (if x then Yes else No) (at level 50).
+Notation "x && y" := (if x then Reduce y else No).
+Notation "x || y" := (if x then Yes else Reduce y).
+
+Definition unwrap {P : Prop} (s : solution P) :=
+match s return if s then P else Prop with
+    | Yes' p => p
+    | _ => True
+end.
