Reflection/CMonRefl.v
@@ -1,21 +1,8 @@
 Add Rec LoadPath "/home/zeimer/Code/Coq".
 
-Require Import ReificationBase.
+Require Import CMon.
 
-Set Implicit Arguments.
-
-Class CMon : Type :=
-{
-    carrier : Type;
-    op : carrier -> carrier -> carrier;
-    neutr : carrier;
-    assoc : forall x y z : carrier, op x (op y z) = op (op x y) z;
-    neutr_l : forall x : carrier, op neutr x = x;
-    neutr_r : forall x : carrier, op x neutr = x;
-    comm : forall x y : carrier, op x y = op y x
-}.
-
-Coercion carrier : CMon >-> Sortclass.
+(*Set Implicit Arguments.*)
 
 Inductive exp (X : CMon) : Type :=
     | Id : exp X
@@ -54,31 +41,6 @@ Proof.
   rewrite ?neutr_l, ?neutr_r; trivial.
 Qed.
 
-Fixpoint expDenoteL {X : CMon} (envX : Env X) (l : list nat) : X :=
-match l with
-    | [] => neutr
-    | h :: t => op (nth h envX neutr) (expDenoteL envX t)
-end.
-
-Lemma expDenoteL_app :
-  forall (X : CMon) (envX : Env X) (l1 l2 : list nat),
-    expDenoteL envX (l1 ++ l2) = op (expDenoteL envX l1) (expDenoteL envX l2).
-Proof.
-  induction l1 as [| h1 t1]; simpl; intros.
-    rewrite neutr_l. reflexivity.
-    rewrite <- assoc, IHt1. reflexivity.
-Qed.
-
-Lemma expDenoteL_Permutation :
-  forall (X : CMon) (envX : Env X) (l1 l2 : list nat),
-    Permutation l1 l2 -> expDenoteL envX l1 = expDenoteL envX l2.
-Proof.
-  induction 1; cbn.
-    reflexivity.
-    rewrite IHPermutation. reflexivity.
-    rewrite !assoc. rewrite (comm (nth y envX neutr)). reflexivity.
-    rewrite IHPermutation1, IHPermutation2. reflexivity.
-Qed.
 
 Fixpoint flatten {X : CMon} (e : exp X) : list nat :=
 match e with
@@ -198,7 +160,7 @@ Arguments fOr [X] _ _.
 Arguments fImpl [X] _ _.
 
 Fixpoint formulaDenote
-  (X : CMon) (envX : Env X) (envP : Env Prop) (f : formula X) : Prop :=
+  {X : CMon} (envX : Env X) (envP : Env Prop) (f : formula X) : Prop :=
 match f with
     | fFalse => False
     | fTrue => True
