Sorting/TrichQuicksort.v
@@ -15,18 +15,18 @@ Local Hint Resolve le_n_S filter_length.
 
 Function htqs (n : nat) (A : TrichDec) (sort : list A -> list A) (l : list A)
   {measure length l} : list A :=
-if @trichb_ltb natlt (length l) (S n)
+if @TrichDec_ltb natlt (length l) (S n)
 then sort l
 else match l with
     | [] => []
     | h :: t =>
-        let '(lo, eq, hi) := trifilter' h t in
+        let '(lo, eq, hi) := trifilter h t in
           htqs n A sort lo ++ h :: eq ++ htqs n A sort hi
 end.
 Proof.
-  intros. rewrite trifilter'_spec in teq1. inversion teq1; subst; cbn.
+  intros. rewrite trifilter_spec in teq1. inversion teq1; subst; cbn.
     pose (filter_length (fun x => h <? x) t). omega.
-  intros. rewrite trifilter'_spec in teq1. inversion teq1; subst; cbn.
+  intros. rewrite trifilter_spec in teq1. inversion teq1; subst; cbn.
     pose (filter_length (fun x => x <? h) t). omega.
 Defined.
 
@@ -37,7 +37,7 @@ Function htqs2
   (n : nat) (A : TrichDec)
   (sort : list A -> list A) (partition : Partition A)
   (l : list A) {measure length l} : list A :=
-    if @trichb_ltb natlt (length l) (S n)
+    if @TrichDec_ltb natlt (length l) (S n)
     then sort l
     else match l with
         | [] => []
@@ -48,24 +48,22 @@ Function htqs2
               htqs2 n A sort partition hi
     end.
 Proof.
-  intros. apply spec_hi in teq1. cbn. omega.
-  intros. apply spec_lo in teq1. cbn. omega.
+  intros. apply spec_hi in teq1. cbn. unfold lt. apply le_n_S. assumption.
+  intros. apply spec_lo in teq1. cbn. unfold lt. apply le_n_S. assumption.
 Defined.
 
 Instance Trifilter (A : TrichDec) : Partition A :=
 {
-    partition := trifilter'
+    partition := trifilter
 }.
 Proof.
-  intros. rewrite trifilter'_spec in H. inversion H; subst; cbn.
-    apply filter_length.
-  intros. rewrite trifilter'_spec in H. inversion H; subst; cbn.
-    apply filter_length.
+  intros. rewrite trifilter_spec in H. inv H.
+  intros. rewrite trifilter_spec in H. inv H.
 Defined.
 
 Definition wut (A : TrichDec) (l : list A) : list A :=
   htqs2 0 A (fun l => l) (Trifilter A) l.
 
-Time Compute wut natlt (cycle 30 testl).
+(*Time Compute wut natlt (cycle 30 testl).
 Time Compute tqs natlt (cycle 3000 testl).
-Time Compute tqs natlt (cycle 1500 [1]).
+Time Compute tqs natlt (cycle 1500 [1]).*)
