Memoization/Memoize.v
@@ -1,0 +1,161 @@
+Add Rec LoadPath "/home/zeimer/Code/Coq".
+
+Require Export RCCBase.
+
+Fixpoint fib (n : nat) : nat :=
+match n with
+    | 0 => 0
+    | 1 => 1
+    | S (S n'' as n') => fib n' + fib n''
+end.
+
+Fixpoint fromTo (a b : nat) : list nat :=
+  if b <? a then [] else
+match b with
+    | 0 => [0]
+    | S b' => fromTo a b' ++ [b]
+end.
+
+Definition test := [0; 1; 2; 3; 4; 5; 6; 7; 8; 9; 10].
+
+Time Compute map fib (fromTo 0 24).
+
+Time Compute fib 24.
+
+Fixpoint find {A : Type} (n : nat) (l : list (nat * A)) : option A :=
+match l with
+    | [] => None
+    | (m, v) :: t => if n =? m then Some v else find n t
+end.
+
+Axiom wut : False.
+
+Instance KVP (A : LinDec) (B : Type) : LinDec :=
+{
+    carrier := A * B;
+    leq p1 p2 := fst p1 ≤ fst p2;
+    leqb p1 p2 := fst p1 <=? fst p2;
+}.
+Proof.
+  all: intros; repeat
+  match goal with
+      | p : _ * _ |- _ => destruct p
+  end; cbn in *; dec.
+  cut False.
+    inversion 1.
+    apply wut.
+Defined.
+
+Fixpoint aux (n : nat) (acc : list (nat * nat)) : nat :=
+match n with
+    | 0 => 0
+    | 1 => 1
+    | S (S n'' as n') =>
+        match find n'' acc with
+            | None =>
+                let a := aux n'' acc in
+                let b := aux n' ((n'', a) :: acc) in a + b
+            | Some a =>
+                match find n' acc with
+                    | None =>
+                        let b := aux n' acc in a + b
+                    | Some b => a + b
+                end
+        end
+end.
+
+Definition fibM n := aux n [(0, 0); (1, 1)].
+
+Compute map fibM test.
+Time Compute fibM 24.
+
+Let list_map := map.
+
+Require Import BTree.
+Require Import BST.
+Require Import TrichDec.
+
+Fixpoint find' {A : TrichDec} {B : Type} (k : A) (t : BTree (KVP A B))
+  : option B :=
+match t with
+    | empty => None
+    | node p l r =>
+        match k <?> fst p with
+            | Lt => find' k l
+            | Eq => Some (snd p)
+            | Gt => find' k r
+        end
+end.
+
+Fixpoint aux' (n : nat) (acc : BTree (KVP natle natle)) : nat :=
+match n with
+    | 0 => 0
+    | 1 => 1
+    | S (S n'' as n') =>
+        match find' n'' acc with
+            | None =>
+                let a := aux' n'' acc in
+                let b := aux' n' (@BTree_ins (KVP natle natle) (n'', a) acc) in a + b
+            | Some a =>
+                match find' n' acc with
+                    | None =>
+                        let b := aux' n' acc in a + b
+                    | Some b => a + b
+                end
+        end
+end.
+
+Time Compute list_map _ _
+  (fun n => aux' n (@fromList (KVP natle natle) [(0, 0); (1, 1)]))
+  (fromTo 0 24).
+
+Definition bind {A : TrichDec} {B : Type} (a : A)
+  (f : A -> BTree (KVP A B) -> B) (acc : BTree (KVP A B))
+  : B * BTree (KVP A B) :=
+match find' a acc with
+    | None => let b := f a acc in (b, @BTree_ins (KVP A B) (a, b) acc)
+    | Some b => (b, acc)
+end.
+
+Fixpoint aux2 (n : nat) (acc : BTree (KVP natle natle)) : nat :=
+match n with
+    | 0 => 0
+    | 1 => 1
+    | S (S n'' as n') =>
+        let '(a, acc') := bind n'' aux2 acc in
+        let '(b, acc'') := bind n' aux2 acc' in a + b
+end.
+
+Definition fib2M n := aux2 n (@fromList (KVP natle natle) [(0, 0); (1, 1)]).
+
+Time Compute list_map _ _ fib (fromTo 0 24).
+Time Compute list_map _ _ fib2M (fromTo 0 24).
+
+Fixpoint wutzor (n : nat) : nat :=
+match n with
+    | 0 => 0
+    | 1 => 0
+    | 2 => 0
+    | 3 => 0
+    | S (S (S (S n4 as n3) as n2) as n1) =>
+        wutzor n4 + wutzor n3 + wutzor n2 + wutzor n1
+end.
+
+Fixpoint wutzor' (n : nat) (acc : BTree (KVP natle natle)) : nat :=
+match n with
+    | 0 => 0
+    | 1 => 0
+    | 2 => 0
+    | 3 => 0
+    | S (S (S (S n4 as n3) as n2) as n1) =>
+        let (x1, acc1) := bind n4 wutzor' acc in
+        let (x2, acc2) := bind n3 wutzor' acc1 in
+        let (x3, acc3) := bind n2 wutzor' acc2 in
+        let (x4, acc4) := bind n1 wutzor' acc3 in x1 + x2 + x3 + x4
+end.
+
+
+Time Compute wutzor 30.
+Time Compute
+  wutzor' 30
+    (@fromList (KVP natle natle) [(0, 0); (1, 0); (2, 0); (3, 0)]).
