Reflection/UCRingRefl.v
@@ -1,0 +1,652 @@
+Add Rec LoadPath "/home/zeimer/Code/Coq".
+
+Require Import UCRing.
+
+Set Implicit Arguments.
+
+(* UCRing expressions. *)
+Inductive exp (X : UCRing) : Type :=
+    | Var : nat -> exp X
+    | Zero : exp X
+    | One : exp X
+    | Add : exp X -> exp X -> exp X
+    | Mul : exp X -> exp X -> exp X
+    | Neg : exp X -> exp X.
+
+Arguments Var [X] _.
+Arguments Zero [X].
+Arguments One [X].
+Arguments Add [X] _ _.
+Arguments Mul [X] _ _.
+Arguments Neg [X] _.
+
+Definition exp_eq_dec {X : UCRing} (e1 e2 : exp X) : {e1 = e2} + {e1 <> e2}.
+Proof.
+  do 2 decide equality.
+Defined.
+
+Fixpoint expDenote {X : UCRing} (env : nat -> X) (e : exp X) : X :=
+match e with
+    | Var n => env n
+    | Zero => 0
+    | One => 1
+    | Add e1 e2 => expDenote env e1 + expDenote env e2
+    | Mul e1 e2 => expDenote env e1 * expDenote env e2
+    | Neg e' => - expDenote env e'
+end.
+
+Function simplifyExp {X : UCRing} (e : exp X) : exp X :=
+match e with
+    | Var n => Var n
+    | Zero => Zero
+    | One => One
+    | Add e1 e2 =>
+        match simplifyExp e1, simplifyExp e2 with
+            | Zero, e2' => e2'
+            | e1', Zero => e1'
+            | e1', Neg e2' =>
+                if exp_eq_dec e1' e2'
+                then Zero
+                else Add e1' (Neg e2')
+            | e1', e2' => Add e1' e2'
+        end
+    | Mul e1 e2 =>
+        match simplifyExp e1, simplifyExp e2 with
+            | Zero, _ => Zero
+            | _, Zero => Zero
+            | One, e2' => e2'
+            | e1', One => e1'
+            | Neg One, e2' => Neg e2'
+            | e1', Neg One => Neg e1'
+            | Add e11 e12, e2' => Add (Mul e11 e2') (Mul e12 e2')
+            | e1', Add e21 e22 => Add (Mul e1' e21) (Mul e1' e22)
+            | Neg e1', Neg e2' => Mul e1' e2'
+            | e1', e2' => Mul e1' e2'
+        end
+    | Neg e' =>
+        match simplifyExp e' with
+            | Zero => Zero 
+            (*| Add e1 e2 => Add (Neg e1) (Neg e2)*)
+            | Mul e1 e2 => Mul (Neg e1) e2
+            | Neg e'' => e''
+            | e'' => Neg e''
+        end
+end.
+
+Theorem simplifyExp_correct :
+  forall (X : UCRing) (env : nat -> X) (e : exp X),
+    expDenote env (simplifyExp e) = expDenote env e.
+Proof.
+  intros. Time functional induction simplifyExp e; cbn; trivial;
+  repeat multimatch goal with
+      | IH : forall _, _ |- _ => rewrite <- ?IH
+      | H : ?a = ?b |- _ => rewrite ?H in *
+      | _ => cbn; rng; autorewrite with lemmas
+  end.
+Qed.
+
+Definition simpExp {X : UCRing} (e : exp X) : exp X :=
+  simplifyExp e.
+
+Lemma simpExp_correct :
+  forall (X : UCRing) (env : nat -> X) (e : exp X),
+    expDenote env (simpExp e) = expDenote env e.
+Proof.
+  unfold simpExp; intros. rewrite !simplifyExp_correct. trivial.
+Qed.
+
+Theorem reflectExp :
+  forall (X : UCRing) (env : nat -> X) (e1 e2 : exp X),
+    expDenote env (simpExp e1) = expDenote env (simpExp e2) ->
+      expDenote env e1 = expDenote env e2.
+Proof.
+  intros. rewrite !simpExp_correct in H. assumption.
+Qed.
+
+(* Some wut proofs. *)
+Inductive NoAdd {X : UCRing} : exp X -> Prop :=
+    | NA_Var : forall n : nat, NoAdd (Var n)
+    | NA_Zero : NoAdd Zero
+    | NA_One : NoAdd One
+    | NA_Mul : forall e1 e2 : exp X,
+        NoAdd e1 -> NoAdd e2 -> NoAdd (Mul e1 e2)
+    | NA_Neg : forall e : exp X, NoAdd e -> NoAdd (Neg e).
+
+Inductive ANF {X : UCRing} : exp X -> Prop :=
+    | ANF_Var : forall n : nat, ANF (Var n)
+    | ANF_Zero : ANF Zero
+    | ANF_One : ANF One
+    | ANF_Add : forall e1 e2 : exp X,
+        ANF e1 -> ANF e2 -> ANF (Add e1 e2)
+    | ANF_Mul : forall e1 e2 : exp X,
+        NoAdd e1 -> NoAdd e2 -> ANF e1 -> ANF e2 -> ANF (Mul e1 e2)
+    | ANF_Neg : forall e : exp X, ANF e -> ANF (Neg e).
+
+Hint Constructors NoAdd ANF.
+
+Ltac inv H := try inversion H; subst; auto.
+
+Ltac inv_NoAdd := repeat
+match goal with
+    | H : NoAdd (Add _ _) |- _ => inv H; clear H
+    | H : NoAdd (Mul _ _) |- _ => inv H; clear H
+    | H : NoAdd (Neg _) |- _ => inv H; clear H
+end.
+
+Theorem simplifyExp_pres_NoAdd :
+  forall (X : UCRing) (e : exp X),
+    NoAdd e -> NoAdd (simplifyExp e).
+Proof.
+  intros. Time functional induction simplifyExp e; try constructor;
+  repeat match goal with
+      | H : NoAdd ?x, IH : NoAdd ?x -> _ |- _ => specialize (IH H)
+      | H : ?x = _, H' : NoAdd ?x |- _ => rewrite H in H'
+      | _ => inv_NoAdd; eauto
+  end.
+Qed.
+
+Ltac inv_ANF := repeat
+match goal with
+    | H : ANF (Add _ _) |- _ => inv H; clear H
+    | H : ANF (Mul _ _) |- _ => inv H; clear H
+    | H : ANF (Neg _) |- _ => inv H; clear H
+end.
+
+Theorem simplifyExp_NoAdd_ANF :
+  forall (X : UCRing) (e : exp X),
+    NoAdd e -> ANF (simplifyExp e).
+Proof.
+  intros. apply simplifyExp_pres_NoAdd in H.
+  Time functional induction simplifyExp e; trivial;
+  repeat match goal with
+      | H : ?x = _, H' : context [ANF ?x] |- _ => rewrite H in H'
+      | H : ?P, IH : ?P -> ?Q |- _ => specialize (IH H)
+      | _ => inv_NoAdd; inv_ANF
+  end;
+  repeat match goal with
+      | H : _ -> ?P |- _ => cut P; auto; clear H; intros
+  end; inv_ANF.
+Qed.
+
+(* Simplification for equality hypotheses *)
+Inductive eqExp (X : UCRing) : Type :=
+    | E : forall e1 e2 : exp X, eqExp X.
+
+Arguments E [X] _ _.
+
+Definition eqExpDenote
+  {X : UCRing} (env : nat -> X) (eq : eqExp X)
+  : Prop :=
+match eq with
+    | E e1 e2 => expDenote env e1 = expDenote env e2
+end.
+
+Function simpHypEq {X : UCRing} (eq : eqExp X) : eqExp X :=
+match eq with
+    | E e1 e2 =>
+        match simplifyExp e1, simplifyExp e2 with
+            | Add e11 e12, Add e21 e22 =>
+                if exp_eq_dec e11 e21
+                then E e12 e22
+                else if exp_eq_dec e12 e22
+                     then E e11 e21
+                     else E (Add e11 e12) (Add e21 e22)
+            | Neg e1', Neg e2' => E e1' e2'
+            | e1', e2' => E e1' e2'
+        end
+end.
+
+Ltac forth :=
+repeat match goal with
+    | |- expDenote ?env ?e1 = expDenote ?env ?e2 =>
+        is_var e1; is_var e2;
+        rewrite <- (simplifyExp_correct env e1),
+                <- (simplifyExp_correct env e2)
+    | H : ?x = _ |- context [?x] => rewrite H; cbn
+end; rng.
+
+Ltac back :=
+repeat match goal with
+    | H : expDenote ?env ?e1 = expDenote ?env ?e2 |- _ =>
+        is_var e1; is_var e2;
+        rewrite <- (simplifyExp_correct env e1),
+                <- (simplifyExp_correct env e2) in H
+    | H : ?x = _ , H' : context [?x] |- _ =>
+        rewrite H in H'; cbn in H'; auto
+end; rng.
+
+Lemma simpHypEq_correct :
+  forall (X : UCRing) (env : nat -> X) (eq : eqExp X),
+    eqExpDenote env (simpHypEq eq) <-> eqExpDenote env eq.
+Proof.
+  intros. functional induction simpHypEq eq; cbn; split; intros.
+    all: try (forth; fail).
+    all: try (back; eapply add_cancel_l + eapply add_cancel_r; eauto; fail).
+    back. apply neg_eq. assumption.
+Qed.
+
+(* Simplification for goal equalities. *)
+Function simpGoalEq {X : UCRing} (eq : eqExp X) : eqExp X :=
+match eq with
+    | E e1 e2 => E (simplifyExp e1) (simplifyExp e2)
+end.
+
+Lemma simpGoalEq_correct :
+  forall (X : UCRing) (env : nat -> X) (eq : eqExp X),
+    eqExpDenote env (simpGoalEq eq) <-> eqExpDenote env eq.
+Proof.
+  intros. functional induction simpGoalEq eq; cbn; split; intros.
+    rewrite ?simplifyExp_correct in H. assumption.
+    rewrite ?simplifyExp_correct. assumption.
+Qed.
+
+(* Formulas. *)
+Inductive formula (X : UCRing) : Type :=
+    | fFalse : formula X
+    | fTrue : formula X
+    | fVar : Prop -> formula X
+    | fEquiv : exp X -> exp X -> formula X
+    | fNot : formula X -> formula X
+    | fAnd : formula X -> formula X -> formula X
+    | fOr : formula X -> formula X -> formula X
+    | fImpl : formula X -> formula X -> formula X.
+
+Arguments fFalse [X].
+Arguments fTrue [X].
+Arguments fVar [X] _.
+Arguments fEquiv [X] _ _.
+Arguments fNot [X] _.
+Arguments fAnd [X] _ _.
+Arguments fOr [X] _ _.
+Arguments fImpl [X] _ _.
+
+Fixpoint formulaDenote
+  {X : UCRing} (env : nat -> X) (p : formula X) : Prop :=
+match p with
+    | fFalse => False
+    | fTrue => True
+    | fVar P => P
+    | fEquiv e1 e2 => expDenote env e1 = expDenote env e2
+    | fNot p' => ~ formulaDenote env p'
+    | fAnd p1 p2 => formulaDenote env p1 /\ formulaDenote env p2
+    | fOr p1 p2 => formulaDenote env p1 \/ formulaDenote env p2
+    | fImpl p1 p2 => formulaDenote env p1 -> formulaDenote env p2
+end.
+
+Function simpFormula {X : UCRing} (f : formula X) : formula X :=
+match f with
+    | fFalse => fFalse
+    | fTrue => fTrue
+    | fVar P => fVar P
+    | fEquiv e1 e2 =>
+        match simpHypEq (E e1 e2) with
+            | E e1' e2' => fEquiv e1' e2'
+        end
+    | fNot f' =>
+        match simpFormula f' with
+            | fFalse => fTrue
+            | fTrue => fFalse
+            | f'' => fNot f''
+        end
+    | fAnd f1 f2 =>
+        match simpFormula f1, simpFormula f2 with
+            | fOr f11 f12, f2' => fOr (fAnd f11 f2') (fAnd f12 f2')
+            | f1', fOr f21 f22 => fOr (fAnd f1' f21) (fAnd f1' f22)
+            | fFalse, _ => fFalse
+            | _, fFalse => fFalse
+            | fTrue, f2' => f2'
+            | f1', fTrue => f1'
+            | f1', f2' => fAnd f1' f2'
+        end
+    | fOr f1 f2 =>
+        match simpFormula f1, simpFormula f2 with
+            | fAnd f11 f12, f2' => fAnd (fOr f11 f2') (fOr f12 f2')
+            | f1', fAnd f21 f22 => fAnd (fOr f1' f21) (fOr f1' f22)
+            | fFalse, f2' => f2'
+            | f1', fFalse => f1'
+            | fTrue, _ => fTrue
+            | _, fTrue => fTrue
+            | f1', f2' => fOr f1' f2'
+        end
+    | fImpl f1 f2 =>
+        match f1 with
+            | fEquiv e1 e2 =>
+                let '(E e1' e2') := simpHypEq (E e1 e2) in
+                  fImpl (fEquiv e1' e2') f2
+            | f1' =>
+                match simpFormula f1' with
+                    | fFalse => fTrue
+                    | fTrue => f2
+                    | fAnd f11 f12 => fImpl f11 (fImpl f12 f2)
+                    | fOr f11 f12 => fAnd (fImpl f11 f2) (fImpl f12 f2)
+                    | f1' => fImpl f1' f2
+                end
+        end
+end.
+
+Theorem simpFormula_correct :
+  forall (X : UCRing) (env : nat -> X) (f : formula X),
+    formulaDenote env (simpFormula f) <-> formulaDenote env f.
+Proof.
+  intros. functional induction simpFormula f; cbn.
+  Time all:
+  repeat match goal with
+      | env : nat -> _, IH : forall env' : nat -> _, _ |- _ =>
+          specialize (IH env)
+      | e : simpFormula ?f = _,
+        IH : formulaDenote _ (simpFormula ?f) <-> _ |- _ =>
+        rewrite <- IH, e; cbn
+  end; try (tauto; fail).
+    assert (eqExpDenote env (simpHypEq (E e1 e2)) =
+           (expDenote env e1' = expDenote env e2')).
+      rewrite e0. cbn. trivial.
+      rewrite <- H. rewrite simpHypEq_correct. cbn. reflexivity.
+    assert (eqExpDenote env (simpHypEq (E e1 e2)) <->
+            eqExpDenote env (E e1' e2')).
+      rewrite e3. tauto.
+      rewrite simpHypEq_correct in H. cbn in H. tauto.
+Qed.
+
+Definition list_eq :
+  forall (l1 l2 : list nat), {l1 = l2} + {l1 <> l2}.
+Proof.
+  do 2 decide equality.
+Defined.
+
+Fixpoint solveFormula
+  {X : UCRing} (env : nat -> X) (f : formula X)
+  : option (formulaDenote env f).
+Proof.
+  destruct f; cbn.
+    apply None.
+    apply Some. trivial.
+    apply None.
+      destruct (exp_eq_dec (simplifyExp e) (simplifyExp e0)).
+        rewrite <- (simplifyExp_correct env e),
+                <- (simplifyExp_correct env e0).
+          rewrite e1. apply Some. trivial.
+        apply None.
+    apply None.
+    destruct (solveFormula X env f1), (solveFormula X env f2).
+      apply Some. split; assumption.
+      1-3: apply None.
+    destruct (solveFormula X env f1).
+      apply Some. left. assumption.
+      destruct (solveFormula X env f2).
+        apply Some. right. assumption.
+        apply None.
+    destruct (solveFormula X env f2).
+      apply Some. intro. assumption.
+      apply None.
+Defined.
+
+Theorem solveFormula_correct :
+  forall (X : UCRing) (env : nat -> X) (f : formula X),
+    (exists p : formulaDenote env f, solveFormula env f = Some p) ->
+      formulaDenote env f.
+Proof.
+  intros. destruct H. assumption.
+Qed.
+
+(* Basic tactics for manipulating lists. *)
+(*Ltac inList x l :=
+match l with
+    | [] => false
+    | x :: _ => true
+    | _ :: ?l' => inList x l'
+end.
+
+Ltac addToList x l :=
+  let b := inList x l in
+match b with
+    | true => l
+    | false => constr:(x :: l)
+end.
+
+Ltac lookup x l :=
+match l with
+    | x :: _ => constr:(0%nat)
+    | _ :: ?l' => let n := lookup x l' in constr:(S n)
+end.*)
+
+Ltac functionalize l X :=
+let rec loop n l' :=
+    match l' with
+        | [] => constr:(fun _ : nat => 0) (* Here 0 : X *)
+        | ?h :: ?t =>
+            let f := loop (S n) t in
+            constr:(fun m : nat => if m =? n then h else f m)
+    end
+in loop 0%nat l.
+
+(* Reification for expressions. *)
+Ltac allVarsExp xs e :=
+match e with
+    | 0 => xs
+    | 1 => xs
+    | ?a + ?b =>
+        let xs' := allVarsExp xs b in allVarsExp xs' a
+    | ?a * ?b =>
+        let xs' := allVarsExp xs b in allVarsExp xs' a
+    | -?a => allVarsExp xs a
+    | _ => addToList e xs
+end.
+
+Ltac reifyExp xs x :=
+match x with
+    | 0 => constr:(Zero)
+    | 1 => constr:(One)
+    | ?a + ?b =>
+        let e1 := reifyExp xs a in
+        let e2 := reifyExp xs b in constr:(Add e1 e2)
+    | ?a * ?b =>
+        let e1 := reifyExp xs a in
+        let e2 := reifyExp xs b in constr:(Mul e1 e2)
+    | -?a =>
+        let e := reifyExp xs a in constr:(Neg e)
+    | ?x =>
+        let n := lookup x xs in constr:(Var n)
+end.
+
+(* Reification of equalities. *)
+Ltac reifyEqv xs a b :=
+  let e1 := reifyExp xs a in
+  let e2 := reifyExp xs b in constr:(E e1 e2).
+
+(* Reification of formulas. *)
+Ltac allVarsFormula xs P :=
+match P with
+    | ?a = ?b =>
+        let xs' := allVarsExp xs b in allVarsExp xs' a
+    | ~ ?P' => allVarsFormula xs P'
+    | ?P1 /\ ?P2 =>
+        let xs' := allVarsFormula xs P2 in allVarsFormula xs' P1
+    | ?P1 \/ ?P2 =>
+        let xs' := allVarsFormula xs P2 in allVarsFormula xs' P1
+    | ?P1 -> ?P2 =>
+        let xs' := allVarsFormula xs P2 in allVarsFormula xs' P1
+    | _ => xs
+end.
+
+Ltac reifyFormula xs P :=
+match P with
+    | False => constr:(fFalse)
+    | True => constr:(fTrue)
+    | ?a = ?b =>
+        let e1 := reifyExp xs a in
+        let e2 := reifyExp xs b in constr:(fEquiv e1 e2)
+    | ~ ?P' =>
+        let e := reifyFormula xs P' in constr:(fNot e)
+    | ?P1 /\ ?P2 =>
+        let e1 := reifyFormula xs P1 in
+        let e2 := reifyFormula xs P2 in constr:(fAnd e1 e2)
+    | ?P1 \/ ?P2 =>
+        let e1 := reifyFormula xs P1 in
+        let e2 := reifyFormula xs P2 in constr:(fOr e1 e2)
+    | ?P1 -> ?P2 =>
+        let e1 := reifyFormula xs P1 in
+        let e2 := reifyFormula xs P2 in constr:(fImpl e1 e2)
+    | _ => constr:(fVar P)
+end.
+
+(* Reflection for equalities in hypotheses and in the goal. *)
+Ltac reflect_eq_hyps := repeat
+match goal with
+    | X : UCRing, H : ?a = ?b |- _ =>
+        let xs := allVarsExp constr:(@nil X) b in
+        let xs' := allVarsExp xs a in
+        let env := functionalize xs' X in
+        let H' := reifyEqv xs' a b in
+          generalize dependent H;
+          match goal with
+              | |- _ -> ?P => change (eqExpDenote env H' -> P)
+          end;
+          let H'' := fresh "H" in intro H'';
+          rewrite <- simpHypEq_correct in H''
+end; cbn in *.
+
+Ltac reflect_eq_goal := cbn; intros;
+match goal with
+    | X : UCRing |- ?a = ?b =>
+        let xs := allVarsExp constr:(@nil X) b in
+        let xs' := allVarsExp xs a in
+        let env := functionalize xs' X in
+        let H' := reifyEqv xs' a b in
+          change (eqExpDenote env H'); apply reflectExp; cbn; try reflexivity
+end.
+
+(* Reflection for formulas. *)
+Ltac reflectFormula :=
+match goal with
+    | X : UCRing |- ?P =>
+        let xs := allVarsFormula constr:(@nil X) P in
+        let env := functionalize xs X in
+        let e := reifyFormula xs P in change (formulaDenote env e);
+          rewrite <- simpFormula_correct
+end.
+
+Ltac ucring_subst := repeat
+multimatch goal with
+    | H : ?x = ?y |- _ => rewrite <- ?H in *
+    | H : ?x = ?x |- _ => clear H
+end; subst.
+
+Ltac solve_goal' :=
+  cbn; reflectFormula; apply solveFormula_correct; cbn; ucring_subst; eauto.
+
+Ltac solve_goal :=
+  try (solve_goal'; fail);
+  fail "Cannot solve the goal".
+
+Ltac ucring := intros; reflect_eq_hyps; subst; reflect_eq_goal.
+
+Section Test.
+
+Variable X : UCRing.
+
+Variables a a' b b' c c' d d' e e' : X.
+
+(* Tests for expression simplifier. *)
+
+(* UCRing axioms for [add]. *)
+Goal a + (b + c) = (a + b) + c.
+Proof. ucring. rng. Qed.
+
+Goal a + b = b + a.
+Proof. ucring. rng. Abort.
+
+Goal 0 + a = a.
+Proof. ucring. Qed.
+
+Goal a + 0 = a.
+Proof. ucring. Qed.
+
+(* UCRing axioms for [neg]. *)
+Goal -a + a = 0.
+Proof. ucring. rng. Qed.
+
+Goal a + (-a) = 0.
+Proof. ucring. Qed.
+
+(* UCRing axioms for [mul]. *)
+Goal a * (b * c) = (a * b) * c.
+Proof. ucring. rng. Qed.
+
+Goal a * b = b * a.
+Proof. ucring. rng. Abort.
+
+Goal 1 * a = a.
+Proof. ucring. Qed.
+
+Goal a * 1 = a.
+Proof. ucring. Qed.
+
+(* Distributivity *)
+Goal a * (b + c) = a * b + a * c.
+Proof. ucring. Qed.
+
+Goal (a + b) * c = a * c + b * c.
+Proof. ucring. Qed.
+
+(* Identities that aren't axioms. *)
+Goal (a + a) - (a + a) = 0.
+Proof. ucring. Qed.
+
+(* --a = a *)
+Goal --a = a.
+Proof. ucring. Qed.
+
+(* 0 * a = 0 *)
+Goal 0 * a = 0.
+Proof. ucring. Qed.
+
+(* a * 0 = 0 *)
+Goal a * 0 = 0.
+Proof. ucring. Qed.
+
+Goal b = b' -> a + (b + c) = (a + b') + c.
+Proof.
+  ucring. rng.
+Qed.
+
+(* Cancel left and right. *)
+Goal a + b = a + b' -> b + c = b' + c.
+Proof.
+  intros. ucring.
+Qed.
+
+Goal a + b = a' + b -> a + c = a' + c.
+Proof.
+  ucring.
+Qed.
+
+Goal -a = -b -> a + c = b + c.
+Proof.
+  ucring.
+Qed.
+
+Goal (a + b) + c = a + (b' + c) -> b = b'.
+Proof.
+  intros. ucring.
+  rewrite add_assoc in H. ucring. ucring. (* TODO *)
+Qed.
+
+Goal False ->  a <> b -> a * a = b * b.
+Proof. solve_goal. Qed.
+
+Goal a = b -> b = c -> c = a -> a = c /\ c + c = b + b.
+Proof.
+  reflectFormula. cbn.
+Abort.
+
+Goal a = b \/ a = c -> a = c \/ a + a = b + b.
+Proof.
+  reflectFormula; cbn.
+Abort.
+
+Goal a = b -> b' = c' -> 2 = 2 \/ c * c = c + (a * c').
+Proof.
+  reflectFormula.
+Abort.
+
+End Test.
