Sorting/TreeSort.v
@@ -14,6 +14,5 @@ Definition treeSort (A : LinDec) (l : list A) : list A :=
 Definition treeSort' (A : LinDec) (l : list A) : list A :=
   toList' (fromList' l).
 
-Time Compute treeSort natle (cycle 100 testl).
-Time Compute treeSort' natle (cycle 100 testl).
-  
+(*Time Compute treeSort natle (cycle 100 testl).
+Time Compute treeSort' natle (cycle 100 testl).*)
