Sorting/TrichQuicksortSpec.v
@@ -4,20 +4,23 @@ Require Import TrichQuicksort.
 
 Set Implicit Arguments.
 
-(* TODO *)
-
-(*Theorem htqs_perm :
+Theorem htqs_perm :
   forall (n : nat) (A : TrichDec) (s : Sort) (l : list A),
     perm A l (htqs n A sort l).
 Proof.
-  intros. functional induction htqs n A sort l; trivial.
+  intros. functional induction htqs n A (@sort s A) l; trivial.
     destruct s; cbn. apply sort_perm.
     apply perm_symm. eapply perm_trans.
       apply perm_front.
       apply perm_cons. unfold perm in *. intro.
-        rewrite count_app, <- IHl0, <- IHl1.
-        rewrite bifilter_spec in e1; inversion_clear e1.
-        rewrite <- count_filter. auto.
+        rewrite !count_app, <- IHl0, <- IHl1.
+        apply trifilter_spec' in e1; inv e1.
+        red in H. specialize (H x). rewrite count_app in H.
+        rewrite plus_assoc, H.
+        replace (fun x0 : A => h <? x0) with
+                (fun x0 : A => negb (x0 <=? h)).
+          rewrite <- !count_filter. trivial.
+          ext x0. rewrite ltb_negb_leqb. trivial.
 Qed.
 
 Theorem htqs_In :
@@ -31,21 +34,24 @@ Theorem htqs_sorted :
   forall (n : nat) (A : TrichDec) (s : Sort) (l : list A),
     sorted A (htqs n A sort l).
 Proof.
-  intros. functional induction htqs n A sort l; trivial.
+  intros. functional induction htqs n A (@sort s A) l; trivial.
     destruct s; cbn. apply sort_sorted.
-    rewrite bifilter_spec in e1; inversion e1; subst. apply sorted_app_all.
+    rewrite trifilter_spec in e1; inv e1. apply sorted_app_all.
       assumption.
-       apply sorted_cons.
-        intros. rewrite htqs_In, filter_In in H; auto. destruct H.
-          destruct (leqb_spec x h).
-            inversion H0.
-            apply TrichDec_not_leq. assumption.
-          assumption.
-      intros. rewrite htqs_In, filter_In in H; auto. destruct H.
-        destruct (leqb_spec x h); intuition.
-Qed.
+      apply sorted_cons; intros.
+        apply in_app_or in H. destruct H.
+          rewrite filter_In in H. destruct H. dec.
+          rewrite htqs_In, filter_In in H. destruct H.
+            unfold TrichDec_ltb in H0. case_eq (h <?> x); intro;
+            rewrite H1 in H0; trich.
+        Search ((_, _) = (_, _)).
+        destruct (filter
+          (fun x : @carrier A => @LinDec_eqb (TrichDec_to_LinDec A) x h) t).
+          cbn. assumption.
+          cbn.
+Admitted. (* TODO *)
 
-Instance Sort_htqs (n : nat) (s : Sort) : Sort :=
+(*Instance Sort_htqs (n : nat) (s : Sort) : Sort :=
 {
     sort := fun A : TrichDec => htqs n A (@sort s A)
 }.
