Structures/CMon.v
@@ -1,0 +1,44 @@
+Add Rec LoadPath "/home/zeimer/Code/Coq".
+
+Require Export RCCBase.
+
+Set Implicit Arguments.
+
+Class CMon : Type :=
+{
+    carrier : Type;
+    op : carrier -> carrier -> carrier;
+    neutr : carrier;
+    assoc : forall x y z : carrier, op x (op y z) = op (op x y) z;
+    neutr_l : forall x : carrier, op neutr x = x;
+    neutr_r : forall x : carrier, op x neutr = x;
+    comm : forall x y : carrier, op x y = op y x
+}.
+
+Coercion carrier : CMon >-> Sortclass.
+
+Fixpoint expDenoteL {X : CMon} (envX : Env X) (l : list nat) : X :=
+match l with
+    | [] => neutr
+    | h :: t => op (nth h envX neutr) (expDenoteL envX t)
+end.
+
+Lemma expDenoteL_app :
+  forall (X : CMon) (envX : Env X) (l1 l2 : list nat),
+    expDenoteL envX (l1 ++ l2) = op (expDenoteL envX l1) (expDenoteL envX l2).
+Proof.
+  induction l1 as [| h1 t1]; simpl; intros.
+    rewrite neutr_l. reflexivity.
+    rewrite <- assoc, IHt1. reflexivity.
+Qed.
+
+Lemma expDenoteL_Permutation :
+  forall (X : CMon) (envX : Env X) (l1 l2 : list nat),
+    Permutation l1 l2 -> expDenoteL envX l1 = expDenoteL envX l2.
+Proof.
+  induction 1; cbn.
+    reflexivity.
+    rewrite IHPermutation. reflexivity.
+    rewrite !assoc. rewrite (comm (nth y envX neutr)). reflexivity.
+    rewrite IHPermutation1, IHPermutation2. reflexivity.
+Qed.
