Structures/TrichDec.v
@@ -1,0 +1,145 @@
+Add Rec LoadPath "/home/zeimer/Code/Coq".
+
+Require Export RCCBase.
+
+Require Export LinDec.
+
+Set Implicit Arguments.
+
+Inductive Ord : Type :=
+    | Lt : Ord
+    | Eq : Ord
+    | Gt : Ord.
+
+Hint Constructors Ord.
+
+Class TrichDec : Type :=
+{
+    carrier : Type;
+    trich_lt : carrier -> carrier -> Prop;
+    trich_lt_irrefl :
+      forall x : carrier, ~ trich_lt x x;
+    trich_lt_antisym :
+      forall x y : carrier, trich_lt x y -> ~ trich_lt y x;
+    trich_lt_trans :
+      forall x y z : carrier, trich_lt x y -> trich_lt y z -> trich_lt x z;
+    trich_lt_trich :
+      forall x y : carrier, trich_lt x y \/ x = y \/ trich_lt y x;
+    trichb : carrier -> carrier -> Ord;
+    trichb_spec1 :
+      forall x y : carrier, trichb x y = Lt <-> trich_lt x y;
+    trichb_spec2 :
+      forall x y : carrier, trichb x y = Eq <-> x = y;
+    trichb_spec3 :
+      forall x y : carrier, trichb x y = Gt <-> trich_lt y x;
+}.
+
+Infix "<" := trich_lt (at level 70).
+Infix "<?>" := trichb (at level 70).
+
+Hint Resolve trich_lt_irrefl trich_lt_antisym trich_lt_trans trich_lt_trich.
+
+Hint Extern 0 =>
+match goal with
+    | H : _ < _ |- _ => apply trich_lt_irrefl in H; contradiction
+end.
+
+Definition TrichDec_ltb {A : TrichDec} (x y : @carrier A) : bool :=
+match x <?> y with
+    | Lt => true
+    | _ => false
+end.
+
+Notation "x <? y" := (TrichDec_ltb x y) (at level 70).
+
+Ltac trich := cbn; unfold TrichDec_ltb; repeat
+match goal with
+    | H : context [match ?x <?> ?y with | _ => _ end] |- _ =>
+        case_eq (x <?> y); intro
+    | |- context [match ?x <?> ?y with | _ => _ end] =>
+        case_eq (x <?> y); intro
+    | H : _ <?> _ = _ |- _ =>
+        rewrite ?trichb_spec1, ?trichb_spec2, ?trichb_spec3 in H
+    | H : ?x < ?y, H' : ?y < ?x |- _ =>
+        pose (trich_lt_antisym x y H); contradiction
+end; dec; cbn; subst; try
+match goal with
+    | H : ?x <> ?x |- _ => contradiction H; reflexivity
+    | H : ?x < ?x |- _ => pose (trich_lt_irrefl x); contradiction
+end; dec.
+
+Instance TrichDec_to_LinDec (A : TrichDec) : LinDec :=
+{
+    carrier := @carrier A;
+    leq x y := ~ trich_lt y x;
+    leqb x y :=
+      match trichb x y with
+          | Gt => false
+          | _ => true
+      end
+}.
+Proof.
+  apply trich_lt_irrefl.
+  intros. decompose [or] (trich_lt_trich x y); trich.
+  intros; intro. decompose [or] (trich_lt_trich z y); trich.
+  intros. decompose [or] (trich_lt_trich x y); trich.
+  intros. case_eq (trichb x y); intro; trich.
+Defined.
+
+Coercion TrichDec_to_LinDec : TrichDec >-> LinDec.
+
+Fixpoint trichb_nat (n m : nat) : Ord :=
+match n, m with
+    | 0, 0 => Eq
+    | 0, _ => Lt
+    | _, 0 => Gt
+    | S n', S m' => trichb_nat n' m'
+end.
+
+Instance natlt : TrichDec :=
+{
+    carrier := nat;
+    trich_lt := Peano.lt;
+    trichb := trichb_nat
+}.
+Proof.
+  1-4: intros; omega.
+  induction x as [| x']; destruct y as [| y']; cbn;
+  split; try (trich; fail).
+    intros. apply lt_n_S. apply IHx'. assumption.
+    rewrite IHx'. apply lt_S_n.
+  induction x as [| x']; destruct y as [| y']; cbn;
+  split; try (trich; fail); intros.
+    f_equal. apply IHx'. assumption.
+    rewrite IHx'. congruence.
+  induction x as [| x']; destruct y as [| y']; cbn;
+  split; try (trich; fail).
+    intros. apply lt_n_S. apply IHx'. assumption.
+    rewrite IHx'. apply lt_S_n.
+Defined.
+
+Lemma trichb_refl :
+  forall (A : TrichDec) (x : A),
+    x <?> x = Eq.
+Proof.
+  intros. rewrite trichb_spec2. trivial.
+Qed.
+
+(*Definition flipOrd (o : Ord) : Ord :=
+match o with
+    | Lt => Gt
+    | Eq => Eq
+    | Gt => Lt
+end.
+
+Lemma trichb_flipOrd :
+  forall (A : TrichDec) (x y : @carrier A), flipOrd (x <?> y) = (y <?> x).
+Proof.
+  intros. unfold flipOrd.
+*)
+
+Lemma ltb_negb_leqb :
+  forall (A : TrichDec) (x y : A), x <? y = negb (y <=? x).
+Proof.
+  intros. trich.
+Qed.
