Structures/UCRing.v
@@ -1,0 +1,159 @@
+Add Rec LoadPath "/home/zeimer/Code/Coq".
+
+Require Export RCCBase.
+
+Set Implicit Arguments.
+
+(* Commutative rings with unit. *)
+Class UCRing : Type :=
+{
+    carrier : Type;
+    add : carrier -> carrier -> carrier;
+    mul : carrier -> carrier -> carrier;
+    zero : carrier;
+    one : carrier;
+    neg : carrier -> carrier;
+    add_assoc: forall x y z : carrier, add (add x y) z = add x (add y z);
+    add_comm : forall x y : carrier, add x y = add y x;
+    zero_l : forall x : carrier, add zero x = x;
+    zero_r : forall x : carrier, add x zero = x;
+    neg_l : forall x : carrier, add (neg x) x = zero;
+    neg_r : forall x : carrier, add x (neg x) = zero;
+    mul_assoc: forall x y z : carrier, mul (mul x y) z = mul x (mul y z);
+    mul_comm : forall x y : carrier, mul x y = mul y x;
+    one_l : forall x : carrier, mul one x = x;
+    one_r : forall x : carrier, mul x one = x;
+    distr_l : forall x y z : carrier,
+      mul x (add y z) = add (mul x y) (mul x z);
+    distr_r : forall x y z : carrier,
+      mul (add x y) z = add (mul x z) (mul y z);
+}.
+
+Notation "x + y" := (add x y).
+Notation "x - y" := (add x (neg y)).
+Notation "x * y" := (mul x y).
+Notation "0" := zero.
+Notation "1" := one.
+Notation "- x" := (neg x).
+
+Coercion carrier : UCRing >-> Sortclass.
+
+(* Basic tactics for rewriting UCRing axioms. *)
+Hint Rewrite @zero_l @zero_r @one_l @one_r @neg_l @neg_r : units.
+Hint Rewrite @add_assoc @mul_assoc : assoc.
+Hint Rewrite <- @add_assoc @mul_assoc : assoc'.
+Hint Rewrite @add_comm @mul_comm : comm.
+Hint Rewrite @distr_l @distr_r : distr.
+Hint Rewrite <- @distr_l @distr_r : distr'.
+
+Ltac rng := cbn; intros; autorewrite with units assoc distr; try congruence.
+Ltac rng' := cbn; intros; autorewrite with units assoc' distr'; try congruence.
+
+(* Basic lemmas. *)
+Lemma add_cancel_l :
+  forall (X : UCRing) (a b b' : X), a + b = a + b' -> b = b'.
+Proof.
+  intros.
+  assert (-a + (a + b) = b); rng'.
+  assert (-a + (a + b') = b'); rng'.
+Qed.
+
+Lemma add_cancel_r :
+  forall (X : UCRing) (a a' b : X), a + b = a' + b -> a = a'.
+Proof.
+  intros. rewrite (add_comm a), (add_comm a') in H.
+  eapply add_cancel_l. exact H.
+Qed.
+
+Lemma neg_neg :
+  forall (X : UCRing) (x : X), --x = x.
+Proof.
+  intros.
+  assert (-x + x = 0); rng.
+  assert (-x + --x = 0); rng.
+  eapply add_cancel_l. rewrite H0. rng.
+Qed.
+
+Lemma minus_a_a :
+  forall (X : UCRing) (a : X), a - a = 0.
+Proof. rng. Qed.
+
+Lemma mul_0_l :
+  forall (X : UCRing) (x : X), 0 * x = 0.
+Proof.
+  intros.
+  assert (0 * x = (0 + 0) * x); rng.
+  rewrite distr_r in H.
+  assert (0 * x - 0 * x = 0 * x + (0 * x - 0 * x)).
+    rewrite <- add_assoc, <- H. trivial.
+    rewrite (minus_a_a X (0 * x)) in H0. rewrite zero_r in H0. rng.
+Qed.
+
+Lemma mul_0_r :
+  forall (X : UCRing) (x : X), x * 0 = 0.
+Proof.
+  intros. rewrite mul_comm. apply mul_0_l.
+Qed.
+
+Lemma minus_zero :
+  forall X : UCRing, -0 = 0.
+Proof.
+Admitted.
+
+Lemma minus_one_l :
+  forall (X : UCRing) (a : X), -(1) * a = -a.
+Proof.
+  intros.
+Admitted.
+
+Lemma minus_one_r :
+  forall (X : UCRing) (a : X), a * -(1) = -a.
+Proof.
+  intros. rewrite mul_comm. apply minus_one_l.
+Qed.
+
+Lemma minus_one_x2 :
+  forall X : UCRing, -(1) * -(1) = 1.
+Proof.
+  intros. rewrite minus_one_l, neg_neg. trivial.
+Qed.
+
+Lemma mul_minus_minus :
+  forall (X : UCRing) (a b : X), -a * -b = a * b.
+Proof.
+  intros. rewrite <- (minus_one_l X a), <- (minus_one_l X b).
+  rewrite <- mul_assoc, (mul_comm (-(1))).
+  rewrite 2!mul_assoc, <- (mul_assoc (-(1))), minus_one_x2. rng.
+Qed.
+
+Lemma neg_add :
+  forall (X : UCRing) (a b : X), -(a + b) = -a + -b.
+Proof.
+  intros.
+  assert (-(a + b) + (a + b) = 0); rng.
+  assert ((-a - b) + (a + b) = 0); rng.
+    rewrite (add_comm a). rewrite <- (add_assoc (-b)). rewrite neg_l. rng.
+    rewrite <- H0 in H. apply add_cancel_r in H. assumption.
+Qed.
+
+Lemma neg_mul :
+  forall (X : UCRing) (a b : X), -(a * b) = (-a) * b.
+Proof.
+  intros. rewrite <- (minus_one_l X (a * b)), <- (minus_one_l X a).
+  rewrite ?mul_assoc. trivial.
+Qed.
+
+Lemma neg_eq :
+  forall (X : UCRing) (a b : X), -a = -b -> a = b.
+Proof.
+  intros. rewrite <- (neg_neg X a), <- (neg_neg X b).
+  rewrite H. trivial.
+Qed.
+
+(* Hint base for lemma rewriting. *)
+Hint Rewrite
+  add_cancel_l add_cancel_r
+  neg_neg neg_add neg_mul neg_eq
+  mul_0_l mul_0_r mul_minus_minus
+  minus_zero minus_one_l minus_one_r minus_one_x2
+  : lemmas.
